We check that the given metric fulfills the four requirements for a
metric, utilising the properties of norms.

\begin{enumerate}
\item $d(\bold{x},\bold{z}) \geq 0$ (non-negativity): As a norm
  $||\cdot||$ is always non-negative, this property is immediate.
\item $d(\bold{x},\bold{z}) = 0 \Leftrightarrow \bold{x}=\bold{z}$ (identity of
  indiscernibles): The norm $||\bold{Mx}-\bold{Mz}||$ is only zero if
  $\bold{Mx}-\bold{Mz}=\bold{0}$ (by the definition of a norm), which
  is again only the case if $\bold{x}=\bold{z}$.  Holds in both
  directions.
\item $d(\bold{x},\bold{z}) = d(\bold{z},\bold{x})$ (symmetry):
  \begin{align*}
    d(\bold{x},\bold{z})&=||\bold{Mx}-\bold{Mz}||&\text{(By def.)} \\
    &=||\bold{Mx}+(-1)\bold{Mz}||&\text{(Rewriting)} \\
    &=||(-1)\bold{Mz}+\bold{Mx}||&\text{(Commutativity of addition)} \\
    &=|-1|||(-1)\bold{Mz}+\bold{Mx}||&\text{(Multiplying by one)} \\
    &=||\bold{Mz}-\bold{Mx}||&\text{(Positive homogeneity of norms)} \\
    &=d(\bold{z},\bold{x})&\text{(By def.)}
\end{align*}
\item $d(\bold{x}, \bold{z}) \leq d(\bold{x}, \bold{y}) + d(\bold{y},
  \bold{z})$ (triangle inequality):
  \begin{align*}
    ||\bold{Mx}-\bold{My}+\bold{My}-\bold{Mz}|| &\leq ||\bold{Mx}-\bold{My}|| + ||\bold{My}-\bold{Mz}||&\text{(By triangle ineq. of norms)}\\
    ||\bold{Mx}-\bold{Mz}|| &\leq ||\bold{Mx}-\bold{My}|| + ||\bold{My}-\bold{Mz}||&\text{(Simplifying terms)}\\
    d(\bold{x}, \bold{z}) &\leq d(\bold{x}, \bold{y}) + d(\bold{y}, \bold{z})&\text{(By def.)}
  \end{align*}
\end{enumerate}\qed